sir/Sir/Proofs/Progress.lean
@@ -21,7 +21,9 @@ def MachineState.StmtReady (s : MachineState) : Stmt → Prop
   | .mallocUninit _ size =>
       ∃ w alloc, s.locals.lookup size = .ok w ∧
         s.globals.memory.IsValidNewAlloc alloc ∧ alloc.size = w.toNat
-  | .mstore32 offset value => s.locals.Defined offset ∧ s.locals.Defined value
+  | .mstore32 offset value =>
+      ∃ w, s.locals.lookup offset = .ok w ∧ s.locals.Defined value ∧
+        s.globals.memory.InBounds w.toNat 32
   | .mload32 _ offset => s.locals.Defined offset
   | .icall _ _ _ => False
 
@@ -221,7 +223,7 @@ theorem progress_stmt_proof
       · exact Generic.Operation.execute_malloc_ok ctx allocation state.globals sizeValue hsize
       · exact hstore
   | mstore32 offset value =>
-      obtain ⟨⟨offsetValue, hoffset⟩, valueValue, hvalue⟩ := hready
+      obtain ⟨offsetValue, hoffset, ⟨valueValue, hvalue⟩, hin⟩ := hready
       let globals' := { state.globals with
         memory := state.globals.memory.writeBytes offsetValue valueValue.toByteArray }
       obtain ⟨locals', hstore⟩ := Locals.bindValues_total state.locals
@@ -233,23 +235,22 @@ theorem progress_stmt_proof
       · simp [Array.mapM_eq_mapM_toList, hoffset, hvalue, bind, Except.bind,
           Functor.map, Except.map, pure, Except.pure]
       · trivial
-      · exact Generic.Operation.execute_mstore32_ok ctx state.globals offsetValue valueValue
+      · exact Generic.Operation.execute_mstore32_ok ctx state.globals offsetValue valueValue hin
       · exact hstore
   | mload32 result offset =>
       obtain ⟨offsetValue, hoffset⟩ := hready
-      let assumed : Vector UInt8 32 := Vector.replicate 32 0
       let resultValue : Word := .ofNat (Evm.fromByteArrayBigEndian
-        (state.globals.memory.readBytes offsetValue ⟨assumed.toArray⟩))
+        (state.globals.memory.readBytes offsetValue 32))
       obtain ⟨locals', hstore⟩ := Locals.bindValues_total state.locals
         (targetVars := #[result]) (vs := #[resultValue]) rfl
       refine ⟨[], ⟨state.globals, locals', next⟩, step_mload32 hdecode ?_⟩
       simp only [decodeSirStatement, Generic.Instruction.Fires]
-      apply fires_of (operation := .mload32) (oracle := assumed) (operands := #[offsetValue])
+      apply fires_of (operation := .mload32) (oracle := ()) (operands := #[offsetValue])
         (results := #[resultValue])
       · simp [Array.mapM_eq_mapM_toList, hoffset, bind, Except.bind,
           Functor.map, Except.map, pure, Except.pure]
       · trivial
-      · exact Generic.Operation.execute_mload32_ok ctx assumed state.globals offsetValue
+      · exact Generic.Operation.execute_mload32_ok ctx state.globals offsetValue
       · exact hstore
   | icall callee args dests => exact hready.elim
 
